src/tls/DataStream.fst
@@ -110,7 +110,7 @@ noeq type state (i:id) =
 (*
  * AR: adding the is_eternal_region refinement to satify the precondition of new_region.
  *)
-val gen: r0:rid{is_eternal_region r0} -> i:id -> (state i * state i)
+val gen: r0:rid{is_eternal_region r0} -> i:id -> ML (state i * state i)
 let gen r0 (i:id) =
   let r = new_region r0 in
   empty_is_well_formed i;
