src/tls/Hashing.fst
@@ -1,7 +1,5 @@
 ﻿(* Copyright (C) 2012--2015 Microsoft Research and INRIA *)
 
-#light "off"
-
 module Hashing
 
 open Platform.Bytes
